MonadClass/MonadReader.v
@@ -1,0 +1,25 @@
+Add Rec LoadPath "/home/zeimer/Code/Coq".
+
+Require Import HSLib.Base.
+Require Import HSLib.MonadBind.Monad.
+
+Class MonadReader
+  (R : Type) (M : Type -> Type) (inst : Monad M) : Type :=
+{
+    ask : M R;
+    local : (R -> R) -> M R -> M R;
+}.
+
+Section MonadState_funs.
+
+Variables
+  (R : Type)
+  (M : Type -> Type)
+  (inst : Monad M)
+  (inst' : MonadReader R M inst).
+
+(** Ask for a function of the environment. *)
+Definition asks {A : Type} (f : R -> A) : M A :=
+  do
+    r <- ask;
+    ret $ f r.
